theories/stlc_mu/lib/cast_emulations.v
@@ -1,39 +1,25 @@
-From fae_gtlc_mu Require Export stlc_mu.lang.
-From fae_gtlc_mu Require Export stlc_mu.typing.
+From fae_gtlc_mu.cast_calculus Require Export types.
+From fae_gtlc_mu.stlc_mu Require Export typing lang lib.fix lib.universe.
+From fae_gtlc_mu.backtranslation Require Export types.
 
-Infix "→" := TArrow : type_scope.
+(** Embeddings *)
 
-Definition Universe_body : type :=
-  (
-    TUnit +
-    (TVar 0 + TVar 0) +
-    (TVar 0 × TVar 0) +
-    (TVar 0 → TVar 0) +
-    (TVar 0)
-  )%type.
+Definition ce_unit_to_unknown : expr :=
+  Lam (Fold (InjL (InjL (InjL (InjL (Var 0)))))).
 
-(* + is left associative; (a + b + c) = ((a + b) + c) *)
-
-Definition Universe : type :=
-  TRec Universe_body.
-
-Definition Universe_unfolded : type :=
-  Universe_body.[Universe/]%type.
-
-Definition Inj_TUnit : expr :=
-  Lam (Fold ((InjL (InjL (InjL (InjL (Var 0))))))).
-
-Definition Inj_TUnit_typed : [] ⊢ₛ Inj_TUnit : (TUnit → Universe).
+Lemma ce_unit_to_unknown_typed Γ τ (G : Ground τ) :
+  Γ ⊢ₛ ce_unit_to_unknown : (TUnit → Universe).
 Proof.
   apply Lam_typed, Fold_typed.
   repeat apply InjL_typed.
   by apply Var_typed.
 Qed.
 
-Definition Inj_TSum : expr :=
+Definition ce_ground_sum_to_unknown : expr :=
   Lam (Fold ((InjL (InjL (InjL (InjR (Var 0))))))).
 
-Definition Inj_TSum_typed : [] ⊢ₛ Inj_TSum : ((Universe + Universe) → Universe)%type.
+Definition ce_ground_sum_to_unknown_typed :
+  [] ⊢ₛ ce_ground_sum_to_unknown : ((Universe + Universe) → Universe)%type.
 Proof.
   apply Lam_typed.
   apply Fold_typed.
@@ -41,20 +27,22 @@ Proof.
   by apply Var_typed.
 Qed.
 
-Definition Inj_TProd : expr :=
+Definition ce_ground_prod_to_unknown : expr :=
   Lam (Fold (InjL (InjL (InjR (Var 0))))).
 
-Definition Inj_TProd_typed : [] ⊢ₛ Inj_TProd : ((Universe × Universe) → Universe).
+Definition ce_ground_prod_to_unknown_typed :
+  [] ⊢ₛ ce_ground_prod_to_unknown : ((Universe × Universe) → Universe).
 Proof.
   apply Lam_typed, Fold_typed.
   repeat apply InjL_typed. asimpl. repeat apply InjR_typed.
   by apply Var_typed.
 Qed.
 
-Definition Inj_TRec : expr :=
+Definition ce_ground_rec_to_unknown  : expr :=
   Lam (Fold (InjR (Unfold (Var 0)))).
 
-Definition Inj_TRec_typed : [] ⊢ₛ Inj_TRec : (TRec Universe → Universe).
+Definition ce_ground_rec_to_unknown_typed :
+  [] ⊢ₛ ce_ground_rec_to_unknown : (TRec Universe → Universe).
 Proof.
   apply Lam_typed. apply Fold_typed.
   apply InjR_typed.
@@ -63,15 +51,13 @@ Proof.
   by apply Var_typed.
 Qed.
 
-Coercion App : expr >-> Funclass.
+(** Extractions *)
 
 Definition Ω : expr :=
   (
     (Lam ((Unfold (Var 0)) (Var 0)))
       (Fold (Lam ((Unfold (Var 0)) (Var 0))))
   ).
-
-Definition Is_Closed τ := forall τ', τ.[τ'/] = τ.
 
 Definition Ω_typed Γ τ : (Is_Closed τ) -> (Γ ⊢ₛ Ω : τ).
 Proof.
@@ -84,32 +70,6 @@ Proof.
     + by apply Var_typed.
   - apply Fold_typed. asimpl. rewrite P.
     apply Lam_typed.
-    apply App_typed with (τ1 := TRec (TVar 0 → τ)).
-    + apply Unfold_typed_help_2 with (τ := (TVar 0 → τ)).
-      asimpl. by rewrite P. by apply Var_typed.
-    + by apply Var_typed.
-Qed.
-
-Definition Fix : expr :=
-  Lam (
-      (Lam (Var 1 ((Unfold (Var 0)) (Var 0))))
-        (Fold (Lam (Var 1 ((Unfold (Var 0)) (Var 0)))))
-  ).
-
-Definition Fix_typed Γ τ : (Is_Closed τ) -> (Γ ⊢ₛ Fix : ((τ → τ) → τ)).
-Proof.
-  intro P.
-  apply Lam_typed.
-  apply App_typed with (τ1 := (TRec (TVar 0 → τ))).
-  - apply Lam_typed.
-    apply App_typed with (τ1 := τ); first by apply Var_typed.
-    apply App_typed with (τ1 := TRec (TVar 0 → τ)).
-    + apply Unfold_typed_help_2 with (τ := (TVar 0 → τ)).
-      asimpl. by rewrite P. by apply Var_typed.
-    + by apply Var_typed.
-  - apply Fold_typed. asimpl. rewrite P.
-    apply Lam_typed.
-    apply App_typed with (τ1 := τ); first by apply Var_typed.
     apply App_typed with (τ1 := TRec (TVar 0 → τ)).
     + apply Unfold_typed_help_2 with (τ := (TVar 0 → τ)).
       asimpl. by rewrite P. by apply Var_typed.
@@ -248,3 +208,96 @@ Proof.
   - by apply Ω_typed.
   - apply Fold_typed. by apply Var_typed.
 Qed.
+
+(** Factorisations *)
+
+Definition up_factorization (f1 f2 : expr) (τ τG : cast_calculus.types.type) (G : Ground τG) (_ : not (Ground τ)) (_ : not (τ = ⋆)) (_ : sym τ τG) : expr :=
+  Lam (f2 (f1 (Var 0))).
+
+Lemma up_factorization_typed {f1 f2 : expr} {τ τG : cast_calculus.types.type} {G : Ground τG} {p1 : not (Ground τ)} {p2 : not (τ = ⋆)} {p3 : sym τ τG} (d1 : forall Γ, Γ ⊢ₛ f1 : (<<τ>> → <<τG>>)) (d2 : forall Γ, Γ ⊢ₛ f2 : (<<τG>> → Universe)) :
+  [] ⊢ₛ up_factorization f1 f2 τ τG G p1 p2 p3 : (<<τ>> → Universe).
+Proof.
+  apply Lam_typed.
+  apply App_typed with (τ1 := << τG >>).
+  apply d2.
+  apply App_typed with (τ1 := << τ >>).
+  apply d1.
+  by apply Var_typed.
+Qed.
+
+Definition down_factorization (f1 f2 : expr) (τ τG : cast_calculus.types.type) (G : Ground τG) (_ : not (Ground τ)) (_ : not (τ = ⋆)) (_ : sym τ τG) : expr :=
+  Lam (f2 (f1 (Var 0))).
+
+Lemma down_factorization_typed {f1 f2 : expr} {τ τG : cast_calculus.types.type} {G : Ground τG} {p1 : not (Ground τ)} {p2 : not (τ = ⋆)} {p3 : sym τ τG} (d1 : forall Γ, Γ ⊢ₛ f1 : (Universe → <<τG>>)) (d2 : forall Γ, Γ ⊢ₛ f2 : (<<τG>> → <<τ>>)) :
+  [] ⊢ₛ up_factorization f1 f2 τ τG G p1 p2 p3 : (Universe → <<τ>>).
+Proof.
+  apply Lam_typed.
+  apply App_typed with (τ1 := << τG >>).
+  apply d2.
+  apply App_typed with (τ1 := Universe).
+  apply d1.
+  by apply Var_typed.
+Qed.
+
+(** Between sums, products, recursive types, arrow types *)
+
+Definition between_sums (τ1 τ2 τ1' τ2' : cast_calculus.types.type) (f1 f2 : expr) : expr :=
+  Lam (Case (Var 0) (InjL (f1 (Var 0))) (InjR (f2 (Var 0)))).
+
+Lemma between_sums_typed (τ1 τ2 τ1' τ2' : cast_calculus.types.type) (f1 f2 : expr) (d1 : ∀ Γ, Γ ⊢ₛ f1 : (<<τ1>> → <<τ1'>>)) (d2 : ∀ Γ, Γ ⊢ₛ f2 : (<<τ2>> → <<τ2'>>)) :
+  [] ⊢ₛ between_sums τ1 τ2 τ1' τ2' f1 f2 : (<<τ1>> + <<τ2>> → <<τ1'>> + <<τ2'>>)%type.
+Proof.
+  apply Lam_typed.
+  apply Case_typed with (τ1 := <<τ1>>) (τ2 := <<τ2>>).
+  by apply Var_typed.
+  constructor. eapply App_typed. apply d1. by apply Var_typed.
+  constructor. eapply App_typed. apply d2. by apply Var_typed.
+Qed.
+
+Definition between_prods (τ1 τ2 τ1' τ2' : cast_calculus.types.type) (f1 f2 : expr) : expr :=
+  Lam (Pair (f1 (Fst (Var 0))) (f2 (Snd (Var 0)))).
+
+Lemma between_prods_typed (τ1 τ2 τ1' τ2' : cast_calculus.types.type) (f1 f2 : expr) (d1 : ∀ Γ, Γ ⊢ₛ f1 : (<<τ1>> → <<τ1'>>)) (d2 : ∀ Γ, Γ ⊢ₛ f2 : (<<τ2>> → <<τ2'>>)) :
+  [] ⊢ₛ between_prods τ1 τ2 τ1' τ2' f1 f2 : ((<<τ1>> × <<τ2>>) → (<<τ1'>> × <<τ2'>>))%type.
+Proof.
+  apply Lam_typed.
+  apply Pair_typed.
+  eapply App_typed. apply d1. econstructor. by apply Var_typed.
+  eapply App_typed. apply d2. econstructor. by apply Var_typed.
+Qed.
+
+(* Definition between_recs (τb τb' : cast_calculus.types.type) (f1 f2 : expr) : expr := *)
+(*   Lam ( *)
+(*       Fix ( *)
+(*           Lam ( *)
+(*               Lam (Fold (f (Unfold (Var 0)))) *)
+(*             ) *)
+(*           ) (Var 0) *)
+(*     ). *)
+
+
+(* Definition between_recs_typed (τb τb' : cast_calculus.types.type) (f1 f2 : expr) : expr := *)
+(*   [] ⊢ₛ  *)
+
+(* From fae_gtlc_mu Require Export stlc_mu.typing. *)
+
+(** Complete definition *)
+
+Fixpoint 𝓕 (τi τf : cast_calculus.types.type) (P : sym τi τf) : expr :=
+  match P with
+  | SymUnit => (Lam (Var 0))
+  | SymUnknownL τ (* ⋆ ~ τ *) => 
+  | SymUnknwonR τ => Unit
+  | SymSum τ1 τ1' τ2 τ2' s1 s2 => Unit
+  | SymProd τ1 τ1' τ2 τ2' s1 s2 => Unit
+  | SymArrow τ1 τ1' τ2 τ2' s1 s2 => Unit
+  end.
+
+
+
+Admitted.
+
+Lemma 𝓕_typed (τi τf : cast_calculus.types.type) :
+  [] ⊢ₛ 𝓕 τi τf : TArrow <<τi>> <<τf>>.
+Admitted.
+
