theories/backtranslation/types.v
@@ -1,0 +1,13 @@
+From fae_gtlc_mu Require Import cast_calculus.types stlc_mu.typing stlc_mu.lib.universe.
+
+Reserved Notation "<< τ >>" (at level 4, τ at next level).
+Fixpoint backtranslate_type (τ : cast_calculus.types.type) : type :=
+  match τ with
+  | cast_calculus.types.TUnit => TUnit
+  | cast_calculus.types.TProd τ1 τ2 => TProd <<τ1>> <<τ2>>
+  | cast_calculus.types.TSum τ1 τ2 => TSum <<τ1>> <<τ2>>
+  | cast_calculus.types.TArrow τ1 τ2 => TArrow <<τ1>> <<τ2>>
+  | cast_calculus.types.TRec τ => TRec <<τ>>
+  | cast_calculus.types.TVar x => TVar x
+  | cast_calculus.types.TUnknown => Universe
+  end where "<< e >>" := (backtranslate_type e).
