theories/stlc_mu/lib/fix.v
@@ -1,0 +1,31 @@
+From fae_gtlc_mu Require Export stlc_mu.lang.
+From fae_gtlc_mu Require Export stlc_mu.typing.
+
+Coercion App : expr >-> Funclass.
+Infix "→" := TArrow : type_scope.
+
+Definition Fix : expr :=
+  Lam (
+      (Lam (Var 1 ((Unfold (Var 0)) (Var 0))))
+        (Fold (Lam (Var 1 ((Unfold (Var 0)) (Var 0)))))
+  ).
+
+Definition Fix_typed Γ τ : (Is_Closed τ) -> (Γ ⊢ₛ Fix : ((τ → τ) → τ)).
+Proof.
+  intro P.
+  apply Lam_typed.
+  apply App_typed with (τ1 := (TRec (TVar 0 → τ))).
+  - apply Lam_typed.
+    apply App_typed with (τ1 := τ); first by apply Var_typed.
+    apply App_typed with (τ1 := TRec (TVar 0 → τ)).
+    + apply Unfold_typed_help_2 with (τ := (TVar 0 → τ)).
+      asimpl. by rewrite P. by apply Var_typed.
+    + by apply Var_typed.
+  - apply Fold_typed. asimpl. rewrite P.
+    apply Lam_typed.
+    apply App_typed with (τ1 := τ); first by apply Var_typed.
+    apply App_typed with (τ1 := TRec (TVar 0 → τ)).
+    + apply Unfold_typed_help_2 with (τ := (TVar 0 → τ)).
+      asimpl. by rewrite P. by apply Var_typed.
+    + by apply Var_typed.
+Qed.
