theories/stlc_mu/lib/universe.v
@@ -1,0 +1,23 @@
+From fae_gtlc_mu Require Export stlc_mu.lang.
+From fae_gtlc_mu Require Export stlc_mu.typing.
+
+Infix "→" := TArrow : type_scope.
+
+Definition Universe_body : type :=
+  (
+    TUnit +
+    (TVar 0 + TVar 0) +
+    (TVar 0 × TVar 0) +
+    (TVar 0 → TVar 0) +
+    (TVar 0)
+  )%type.
+
+(* + is left associative; (a + b + c) = ((a + b) + c) *)
+
+Definition Universe : type :=
+  TRec Universe_body.
+
+Definition Universe_unfolded : type :=
+  Universe_body.[Universe/]%type.
+
+(* Coercion App : expr >-> Funclass. *)
